theories/memory.v
@@ -1,175 +1,86 @@
-(** a typeclass for memory, with two implementations:
- - a list-based implementation
- - a lazy sparse array-based implementation *)
+(** a typeclass for a Wasm memory *)
 (* (C) J. Pichon - see LICENSE.txt *)
 
+From mathcomp Require Import ssreflect eqtype.
+Require Import BinNat.
+From Wasm Require Import bytes.
+
+(*
 From mathcomp Require Import ssreflect eqtype seq.
 Require Import BinNat Lia.
 From Wasm Require Import numerics bytes array.
+*)
 
-Class Memory (Mem_t : Type) := {
-  mem_eqtype : unit; (* TODO: fix this *)
+Module Memory.
+
+Definition mem_make_t Mem_t := byte -> N -> Mem_t.
+Definition mem_length_t Mem_t := Mem_t -> N.
+Definition mem_grow_t Mem_t := N -> Mem_t -> Mem_t.
+Definition mem_lookup_t Mem_t := N -> Mem_t -> option byte.
+Definition mem_update_t Mem_t := N -> byte -> Mem_t -> option Mem_t.
+
+Definition mem_ax_lookup_out_of_bounds
+  (Mem_t : Type)
+  (mem_make : mem_make_t Mem_t)
+  (mem_length : mem_length_t Mem_t)
+  (mem_grow : mem_grow_t Mem_t)
+  (mem_lookup : mem_lookup_t Mem_t)
+  (mem_update : mem_update_t Mem_t) :=
+  forall mem i, N.ge i (mem_length mem) -> mem_lookup i mem = None.
+
+Definition mem_ax_lookup_make
+  (Mem_t : Type)
+  (mem_make : mem_make_t Mem_t)
+  (mem_length : mem_length_t Mem_t)
+  (mem_grow : mem_grow_t Mem_t)
+  (mem_lookup : mem_lookup_t Mem_t)
+  (mem_update : mem_update_t Mem_t) :=
+  forall i len b, N.lt i len -> mem_lookup i (mem_make b len) = Some b.
+
+Definition mem_ax_lookup_update
+  (Mem_t : Type)
+  (mem_make : mem_make_t Mem_t)
+  (mem_length : mem_length_t Mem_t)
+  (mem_grow : mem_grow_t Mem_t)
+  (mem_lookup : mem_lookup_t Mem_t)
+  (mem_update : mem_update_t Mem_t) :=
+  forall mem mem' i b, N.lt i (mem_length mem) -> Some mem' = mem_update i b mem -> mem_lookup i mem' = Some b.
+
+Definition mem_ax_lookup_skip
+  (Mem_t : Type)
+  (mem_make : mem_make_t Mem_t)
+  (mem_length : mem_length_t Mem_t)
+  (mem_grow : mem_grow_t Mem_t)
+  (mem_lookup : mem_lookup_t Mem_t)
+  (mem_update : mem_update_t Mem_t) :=
+  forall mem mem' i i' b, i <> i' -> Some mem' = mem_update i' b mem -> mem_lookup i mem' = mem_lookup i mem.
+
+Definition mem_ax_length_constant_update
+  (Mem_t : Type)
+  (mem_make : mem_make_t Mem_t)
+  (mem_length : mem_length_t Mem_t)
+  (mem_grow : mem_grow_t Mem_t)
+  (mem_lookup : mem_lookup_t Mem_t)
+  (mem_update : mem_update_t Mem_t) :=
+  forall i b mem mem', Some mem' = mem_update i b mem -> mem_length mem' = mem_length mem.
+
+Record mixin_of (Mem_t : eqType) := Mixin {
   mem_make : byte -> N -> Mem_t;
   mem_length : Mem_t -> N;
-  mem_grow : N -> Mem_t -> Mem_t;
-  mem_lookup : N -> Mem_t -> option byte;
+  mem_grow : mem_grow_t Mem_t;
+  mem_lookup : mem_lookup_t Mem_t;
   mem_update : N -> byte -> Mem_t -> option Mem_t;
-  mem_ax_lookup_out_of_bounds : forall mem n, N.ge n (mem_length mem) -> mem_lookup n mem = None;
-  mem_ax_lookup_make : forall n len b, N.lt n len -> mem_lookup n (mem_make b len) = Some b;
-  mem_ax_lookup_update : forall mem mem' n b, N.lt n (mem_length mem) -> Some mem' = mem_update n b mem -> mem_lookup n mem' = Some b;
-  mem_ax_lookup_skip : forall mem mem' n n' b, n <> n' -> Some mem' = mem_update n' b mem -> mem_lookup n mem' = mem_lookup n mem;
-  (* TODO: probably need more, like length constancy *)
+  _ : mem_ax_lookup_out_of_bounds Mem_t mem_make mem_length mem_grow mem_lookup mem_update;
+  _ : mem_ax_lookup_make Mem_t mem_make mem_length mem_grow mem_lookup mem_update;
+  _ : mem_ax_lookup_update Mem_t mem_make mem_length mem_grow mem_lookup mem_update;
+  _ : mem_ax_lookup_skip Mem_t mem_make mem_length mem_grow mem_lookup mem_update;
+  _ : mem_ax_length_constant_update Mem_t mem_make mem_length mem_grow mem_lookup mem_update;
 }.
 
-Module Byte_Index <: array.Index_Sig.
-Definition Index := N.
-Definition Value := byte.
-Definition index_eqb := N.eqb.
-Definition index_eqb_eqP : Equality.axiom index_eqb.
-apply ssrnat.eq_binP.
-Defined.
-End Byte_Index.
+Notation class_of := mixin_of.
 
-Module Byte_array := array.Make Byte_Index.
+Structure type : Type := Pack {sort :> eqType; class : class_of sort; }.
 
-Record data_vec : Type := {
-  dv_length : N;
-  dv_array : Byte_array.array;
-}.
+End Memory.
 
-Program Instance data_vec_Memory : Memory data_vec := {
-mem_make := (fun v len => {| dv_length := len; dv_array := Byte_array.make v |} );
-mem_length := (fun dv => dv.(dv_length));
-mem_grow := (fun len_delta dv => {| dv_length := dv.(dv_length) + len_delta; dv_array := dv.(dv_array) |});
-mem_lookup := (fun i dv => if N.ltb i dv.(dv_length) then Some (Byte_array.get dv.(dv_array) i) else None);
-mem_update := (fun i v dv => if N.ltb i dv.(dv_length) then Some {| dv_length := dv.(dv_length); dv_array := Byte_array.set dv.(dv_array) i v |} else None);
-}.
-Next Obligation.
-(* TODO: fragile names *)
-have Hrw: (N.ltb n (dv_length mem) = false); last by rewrite Hrw.
-apply/N.ltb_ge.
-lia.
-Defined.
-Next Obligation.
-apply N.ltb_lt in H.
-by rewrite H.
-Defined.
-Next Obligation.
-apply N.ltb_lt in H.
-rewrite H in H0.
-case: mem' H0 => dv_len dv_arr [Hlen Harr].
-rewrite /= Hlen H Harr.
-f_equal.
-apply Byte_array.get_set.
-Defined.
-Next Obligation.
-case: mem' H0 => dv_len dv_arr /=.
-destruct (N.ltb n' (dv_length mem)) eqn:H2. (* TODO: style? *)
-{ move => [Hlen Harr].
-  rewrite /= Hlen.
-  case (N.ltb n (dv_length mem)); last done.
-  f_equal.
-  rewrite Harr.
-  rewrite Byte_array.get_skip; first by reflexivity.
-  case: (Byte_Index.index_eqb_eqP n n'). (* TODO: this is silly *)
-  { move => Hctr. exfalso.
-  apply: H. apply Hctr. }
-  { done. } 
-}  
-{ move => Hdisc. discriminate Hdisc. }
-Defined.
-
-Record data_list : Type := {
-  dl_init : byte;
-  dl_data : list byte;
-}.
-
-Lemma nth_repeat :
- forall A b i len, i < len ->
- @List.nth_error A (List.repeat b len) i = Some b.
-Proof.
-move => A b.
-elim => [|i].
-{ case => [|len]; first by lia.
-  by move => _. }
-{ move => IH len.
-  case: len => [|len'].
-  { move => Hctr.
-    exfalso.
-    lia. }
-  { move => Hlen /=.
-    apply: IH.
-    lia. } }
-Qed.
-
-Lemma foo : forall A (l : list A) i b,
-i < List.length l ->
-List.nth_error
-  (take i l ++ b :: drop (i+1) l) i =
-Some b.
-Proof.
-move => A.
-elim => [|x l].
-{ move => i b /= Hlen.
-  exfalso.
-  lia. }
-{ move => IH.
-  case => [|i]; first by reflexivity.
-  move => b /= Hlen.
-  have Hlen': i < length l by lia.
-  by apply: IH.
-}
-Qed.
-
-Lemma bar : forall A n n' (l : list A) v,
-n <> n' -> n' < List.length l ->
-List.nth_error (take n' l ++ v :: drop (n' + 1) l) n =
-List.nth_error l n.
-Proof.
-Admitted.
-
-Program Instance data_list_Memory : Memory data_list := {
-mem_make := (fun v len => {| dl_init := v; dl_data := List.repeat v (N.to_nat len) |});
-mem_length := (fun dl => N.of_nat (List.length dl.(dl_data)));
-mem_grow := (fun len_delta dl => {| dl_init := dl.(dl_init); dl_data := dl.(dl_data) ++ List.repeat dl.(dl_init) (N.to_nat len_delta) |});
-mem_lookup := (fun i dl => List.nth_error dl.(dl_data) (N.to_nat i));
-mem_update :=
-  (fun i v dl =>
-   if N.ltb i (N.of_nat (List.length dl.(dl_data)))
-   then Some {| dl_init := dl.(dl_init);
-                dl_data := take (N.to_nat i) dl.(dl_data) ++ [::v] ++ drop (N.to_nat i+1) dl.(dl_data) |}
-   else None);
-}.
-Next Obligation.
-apply (List.nth_error_None mem.(dl_data) (N.to_nat n)).
-apply N.ge_le in H.
-move: H.
-set x := (length (dl_data mem)).
-move => H.
-lia.
-Defined.
-Next Obligation.
-apply: nth_repeat.
-lia.
-Defined.
-Next Obligation.
-apply N.ltb_lt in H.
-rewrite H in H0.
-case: mem' H0 => init_ data_ [Hinit Hdata].
-rewrite Hinit Hdata /= {init_ data_ Hinit Hdata}.
-set nn := N.to_nat n.
-have Hx: nn < length (dl_data mem).
-apply N.ltb_lt in H.
-lia.
-by apply: foo.
-Defined.
-Next Obligation.
-case: mem' H0 => init_ data_.
-case_eq (N.ltb n' (N.of_nat (length (dl_data mem)))); last by discriminate.
-move => Hlen [Hinit Hdata] /=.
-rewrite Hdata => {Hdata}.
-apply: bar.
-lia.
-apply N.ltb_lt in Hlen.
-lia.
-Defined.
+Notation memoryType := Memory.type.
