theories/memory_array.v
@@ -1,0 +1,144 @@
+(** an implementation of Wasm memory based on a sparse array *)
+(* (C) J. Pichon - see LICENSE.txt *)
+
+From mathcomp Require Import ssreflect eqtype.
+Require Import BinNat Lia.
+From Wasm Require Import numerics bytes array memory.
+
+Module Byte_Index <: array.Index_Sig.
+  Definition Index := N.
+  Definition Value := byte.
+  Definition index_eqb := N.eqb.
+  Definition index_eqb_eqP : Equality.axiom index_eqb.
+  apply ssrnat.eq_binP.
+  Defined.
+End Byte_Index.
+
+Module Byte_array := array.Make Byte_Index.
+
+(** An implementation of Wasm memory based on a sparse array
+*)
+Record memory_array : Type := {
+  ma_length : N;
+  ma_array : Byte_array.array;
+}.
+
+Definition mem_make : Memory.mem_make_t memory_array :=
+  fun v len => {| ma_length := len; ma_array := Byte_array.make v |}.
+
+Definition mem_length : Memory.mem_length_t memory_array :=
+  fun ma => ma.(ma_length).
+
+Definition mem_grow : Memory.mem_grow_t memory_array :=
+  fun len_delta ma =>
+    {|
+      ma_length := ma.(ma_length) + len_delta;
+      ma_array := ma.(ma_array)
+    |}.
+
+Definition mem_lookup  : Memory.mem_lookup_t memory_array :=
+  fun i ma =>
+    if N.ltb i ma.(ma_length) then Some (Byte_array.get ma.(ma_array) i)
+    else None.
+
+Definition mem_update : Memory.mem_update_t memory_array :=
+  fun i v ma =>
+    if N.ltb i ma.(ma_length) then
+      Some
+        {|
+          ma_length := ma.(ma_length);
+          ma_array := Byte_array.set ma.(ma_array) i v |}
+    else None.
+
+Lemma memory_array_ax_lookup_out_of_bounds :
+  Memory.mem_ax_lookup_out_of_bounds memory_array mem_make mem_length mem_grow mem_lookup mem_update.
+Proof.
+move => mem i H.
+rewrite /mem_lookup.
+have Hrw: (N.ltb i (ma_length mem) = false); last by rewrite Hrw.
+rewrite /mem_length in H.
+apply/N.ltb_ge.
+lia.
+Qed.
+
+Lemma memory_array_ax_lookup_make : Memory.mem_ax_lookup_make memory_array mem_make mem_length mem_grow mem_lookup mem_update.
+Proof.
+move => i len b H.
+rewrite /mem_lookup.
+apply N.ltb_lt in H.
+by rewrite H.
+Qed.
+
+Lemma memory_array_ax_lookup_update : Memory.mem_ax_lookup_update memory_array mem_make mem_length mem_grow mem_lookup mem_update.
+Proof.
+move => mem mem' i b H H0.
+apply N.ltb_lt in H.
+rewrite /mem_update H in H0.
+case: mem' H0 => ma_len ma_arr [Hlen Harr].
+rewrite /mem_lookup /= Hlen H Harr.
+f_equal.
+apply Byte_array.get_set.
+Qed.
+
+Lemma memory_array_ax_lookup_skip :
+  Memory.mem_ax_lookup_skip memory_array mem_make mem_length mem_grow mem_lookup mem_update.
+Proof.
+move => mem mem' i i' b Hii'.
+rewrite /mem_lookup /mem_update.
+case: mem' => ma_len ma_arr /=.
+destruct (N.ltb i' (ma_length mem)) eqn:H2. (* TODO: style? *)
+{ move => [Hlen Harr].
+  rewrite /= Hlen.
+  case (N.ltb i (ma_length mem)); last done.
+  f_equal.
+  rewrite Harr.
+  rewrite Byte_array.get_skip; first by reflexivity.
+  case: (Byte_Index.index_eqb_eqP i i'). (* TODO: this is silly *)
+  { move => Hctr. exfalso.
+  apply: Hii'. apply Hctr. }
+  { done. } 
+}  
+{ move => Hdisc. discriminate Hdisc. }
+Qed.
+
+Lemma memory_array_ax_length_constant_update :
+  Memory.mem_ax_length_constant_update memory_array mem_make mem_length mem_grow mem_lookup mem_update.
+Proof.
+move => i b mem mem'.
+rewrite /mem_update /mem_length.
+case: mem => ma_len ma_arr.
+case: mem' => ma_len' ma_arr'.
+rewrite /=.
+destruct (N.ltb i ma_len) eqn:H2. (* TODO: style? *)
+{
+move => [Hlen Harr].
+assumption.
+}
+{ move => Hdisc. discriminate Hdisc. }
+Qed.
+
+Definition eqmemory_array (ma1 ma2 : memory_array) : bool.
+(* TODO *)
+Admitted.
+
+Definition eqmemory_arrayP : Equality.axiom eqmemory_array.
+(* TODO *)
+Admitted.
+
+Definition memory_array_eqMixin := Equality.Mixin eqmemory_arrayP.
+Canonical memory_array_eqType := @Equality.Pack memory_array memory_array_eqMixin.
+
+Definition array_memoryMixin :=
+  Memory.Mixin
+    memory_array
+    mem_make
+    mem_length
+    mem_grow
+    mem_lookup
+    mem_update
+    memory_array_ax_lookup_out_of_bounds
+    memory_array_ax_lookup_make
+    memory_array_ax_lookup_update
+    memory_array_ax_lookup_skip
+    memory_array_ax_length_constant_update.
+Canonical array_memoryType := @Memory.Pack memory_array_eqType array_memoryMixin.
